Draft proof

TwoPhaseCommit.thy
@@ -7,6 +7,11 @@ datatype pa_state = PaInit | PaReady | PaCommit | PaAbort
 
 type_synonym system_state = "co_state * (nat \<Rightarrow> pa_state)"
 
+fun consistent_pa_states :: "pa_state \<Rightarrow> pa_state \<Rightarrow> bool" where
+  "consistent_pa_states PaCommit PaAbort = False"
+| "consistent_pa_states PaAbort PaCommit = False"
+| "consistent_pa_states _ _ = True"
+
 definition init :: "nat \<Rightarrow> system_state" where
   "init N = (CoInit, \<lambda>i. if i < N then PaInit else undefined)"
 
@@ -41,7 +46,7 @@ fun pa_abort :: "nat \<Rightarrow> nat \<Rightarrow> system_state \<Rightarrow> 
     else
       (c, ps)
   )"
-
+ 
 
 fun pa_act :: "nat \<Rightarrow> system_state \<Rightarrow> system_state" where
   "pa_act N (CoWait, ps) = (CoWait, \<lambda>i. if i < N \<and> ps i = PaInit then PaReady else ps i)"
@@ -50,56 +55,220 @@ fun pa_act :: "nat \<Rightarrow> system_state \<Rightarrow> system_state" where
 | "pa_act N (c, ps) = (c, ps)"
 
 inductive valid_sys :: "system_state \<Rightarrow> nat \<Rightarrow> bool" where
-  "valid_sys (init N) N"
+  "valid_sys (init N) N"  (*1*)
 | "\<lbrakk>valid_sys s N ;
    s' = co_abort s\<rbrakk> \<Longrightarrow> 
-   valid_sys s' N"
+   valid_sys s' N"        (*2*)
 | "\<lbrakk>valid_sys s N;
    s' = co_commit s \<rbrakk> \<Longrightarrow> 
-   valid_sys s' N"
+   valid_sys s' N"        (*3*)
 | "\<lbrakk>valid_sys s N;
     s' = co_act N s\<rbrakk> \<Longrightarrow>
-    valid_sys s' N"
+    valid_sys s' N"       (*4*)
 | "\<lbrakk>valid_sys s N;
     s' = pa_act N s\<rbrakk> \<Longrightarrow>
-    valid_sys s' N"
+    valid_sys s' N"       (*5*)
 | "\<lbrakk>valid_sys s N;
     x < N;
     s' = pa_abort N x s\<rbrakk> \<Longrightarrow>
-    valid_sys s' N"
+    valid_sys s' N"       (*6*)
 
-(*
-lemma first_phase_no_commit:
+
+lemma co_act_ps_unchanged:
+  assumes "co_act N (c, p) = (c', p')"
+  shows "p = p'"
+  by (smt (verit, best) assms co_act.simps(1) co_act.simps(2) co_act.simps(3) co_act.simps(4) co_state.exhaust prod.inject)
+
+
+lemma co_init_pa_init_or_abort:
   assumes "valid_sys s N"
-    and "(fst s = CoInit) \<or> (fst s = CoWait)"
-  shows "\<not>(\<exists>x < N. ((snd s) x) = PaCommit)"
-  sorry
-*)
+    and "fst s = CoInit"
+    and "x < N"
+  shows "((snd s) x = PaInit) \<or> ((snd s) x = PaAbort)"
+using assms proof (induction s N arbitrary: x rule: valid_sys.induct)
+  case (1 N)
+  then show ?case
+    using init_def by force
+next
+  case (2 s N s')
+  then show ?case
+    by (metis co_abort.elims co_state.distinct(5) split_pairs)
+next
+  case (3 s N s')
+  then show ?case
+    by (metis co_commit.elims co_commit.simps(4) co_state.distinct(1) split_pairs)
+next
+  case (4 s N s')
+  then show ?case 
+    by (smt (verit, ccfv_threshold) co_act.elims co_state.distinct(5) co_state.simps(4) fst_conv)
+next
+  case (5 s N s')
+  then show ?case 
+    by (smt (verit) co_state.exhaust eq_fst_iff pa_act.simps(1) 
+        pa_act.simps(2) pa_act.simps(3) pa_act.simps(4))
+next
+  case (6 s N x s')
+  then show ?case
+    by (metis (no_types, lifting) fun_upd_other fun_upd_same pa_abort.simps split_pairs)
+qed 
 
-lemma co_commit_pa_no_abort:
+lemma co_wait_pa_init_or_abort_or_ready:
+  assumes "valid_sys s N"
+    and "fst s = CoWait"
+    and "x < N"
+  shows "((snd s) x = PaInit) \<or> ((snd s) x = PaAbort) \<or> ((snd s) x = PaReady)"
+using assms proof (induction s N arbitrary: x rule: valid_sys.induct)
+  case (1 N)
+  then show ?case
+    by (simp add: init_def)
+next
+  case (2 s N s')
+  then show ?case 
+    by (smt (verit, best) co_abort.simps(1) co_abort.simps(2) co_abort.simps(3) co_abort.simps(4) 
+        co_init_pa_init_or_abort co_state.exhaust split_pairs)
+next
+  case (3 s N s')
+  then show ?case 
+    by (smt (verit, ccfv_threshold) co_commit.simps(1) co_commit.simps(2) co_commit.simps(3) 
+        co_commit.simps(4) co_init_pa_init_or_abort co_state.exhaust split_pairs)
+next
+  case (4 s N s')
+  then show ?case 
+    by (smt (verit, ccfv_SIG) co_act.simps(2) co_act.simps(3) co_act.simps(4) co_act_ps_unchanged co_state.exhaust prod.collapse)
+next
+  case (5 s N s')
+  then show ?case
+    by (smt (verit, ccfv_SIG) fst_conv pa_act.elims pa_act.simps(1) snd_conv)
+next
+  case (6 s N x s')
+  then show ?case 
+    by (smt (verit, ccfv_SIG) fun_upd_other fun_upd_same pa_abort.simps split_pairs)
+qed
+
+
+
+lemma co_commit_pa_commit_or_ready:
   assumes "valid_sys s N"
     and "fst s = CoCommit"
-  shows "\<not>(\<exists>x < N. ((snd s) x) = PaAbort)"
-  sorry
+    and "x < N"
+  shows "(((snd s) x) = PaCommit) \<or> (((snd s) x) = PaReady)"
+using assms proof (induction s N arbitrary: x rule: valid_sys.induct)
+  case (1 N)
+  then show ?case
+    by (simp add: init_def)
+next
+  case (2 s N s')
+  then show ?case
+    by (metis (full_types) co_abort.elims co_state.distinct(11) co_state.simps(8) fst_conv)
+next
+  case (3 s N s')
+  then show ?case 
+    by (metis co_commit.cases co_commit.simps(1) co_commit.simps(2) co_commit.simps(3) 
+        co_commit.simps(4) co_state.distinct(7) split_pairs)
+next
+  case (4 s N s')
+  have "snd s' = snd s"
+    using co_act_ps_unchanged
+    by (metis "4.hyps"(2) prod.collapse)
+  have "fst s' = CoCommit"
+    by (simp add: "4.prems"(1))
+  then show ?case 
+    by (smt (verit, best) "4.IH" "4.hyps"(2) "4.prems"(2) \<open>snd s' = snd s\<close> co_act.simps(1) co_act.simps(2) co_act.simps(4) co_state.distinct(11) co_state.exhaust split_pairs)
+next
+  case (5 s N s')
+  then show ?case 
+    by (smt (verit, ccfv_SIG) co_state.exhaust pa_act.simps(1) pa_act.simps(2) pa_act.simps(3) 
+        pa_act.simps(4) prod.collapse split_pairs)
+next
+  case (6 s N x s')
+  then show ?case 
+    by (metis pa_abort.simps pa_state.distinct(1) pa_state.distinct(3) split_pairs)
+qed 
 
-lemma co_abort_pa_no_commit:
+corollary co_commit_pa_no_abort:
+  assumes "valid_sys s N"
+    and "fst s = CoCommit"
+    and "x < N"
+  shows "((snd s) x) \<noteq> PaAbort"
+  using assms(1) assms(2) assms(3) co_commit_pa_commit_or_ready by fastforce
+
+
+lemma co_abort_pa_init_or_ready_abort:
   assumes "valid_sys s N"
     and "fst s = CoAbort"
-  shows "\<not>(\<exists>x < N. ((snd s) x) = PaCommit)"
-  sorry
+    and "x < N"
+  shows "(((snd s) x) = PaInit) \<or> (((snd s) x) = PaReady) \<or>
+        (((snd s) x) = PaAbort)"
+  using assms proof (induction s N arbitrary: x rule: valid_sys.induct)
+  case (1 N)
+  then show ?case
+    by (simp add: init_def)
+next
+  case (2 s N s')
+(* apply case distinction, if fst s is CoAbort or CoWait *)
+  then show ?case
+    by (smt (verit, del_insts) co_abort.simps(1) co_abort.simps(2) co_abort.simps(3) 
+        co_abort.simps(4) co_init_pa_init_or_abort co_state.exhaust split_pairs)
+next
+  case (3 s N s')
+  then show ?case 
+    by (smt (verit, best) co_commit.simps(1) co_commit.simps(2) co_commit.simps(3) 
+        co_commit.simps(4) co_state.distinct(9) co_state.exhaust split_pairs)
+next
+  case (4 s N s')
+  then show ?case 
+    by (smt (verit, ccfv_SIG) co_act.simps(2) co_act.simps(3) co_act_ps_unchanged co_state.exhaust co_wait_pa_init_or_abort_or_ready prod.collapse)
+next
+  case (5 s N s')
+  then show ?case 
+    by (smt (verit, del_insts) fst_conv pa_act.elims pa_act.simps(3) snd_conv)
+next
+  case (6 s N x s')
+  then show ?case 
+    by (smt (verit, ccfv_threshold) fun_upd_other fun_upd_same 
+        pa_abort.simps pa_state.exhaust pa_state.simps(12) split_pairs)
+qed
+  
+
+corollary co_abort_pa_no_commit:
+  assumes "valid_sys s N"
+    and "fst s = CoAbort"
+    and "x < N"
+  shows "((snd s) x) \<noteq> PaCommit"
+  using assms(1) assms(2) assms(3) co_abort_pa_init_or_ready_abort by fastforce
 
 lemma pa_init_pa_no_commit:
   assumes "valid_sys s N"
     and "\<exists>x < N. ((snd s) x) = PaInit"
-  shows "\<not>(\<exists>y < N. ((snd s) y) = PaCommit)"
-  sorry
+    and "y < N"
+  shows "((snd s) y) \<noteq> PaCommit"
+  using assms proof (induction s N arbitrary: y rule: valid_sys.induct)
+  case (1 N)
+  then show ?case
+    by (simp add: init_def)
+next
+  case (2 s N s')
+  then show ?case
+    by (smt (verit, best) co_abort.simps(1) co_abort.simps(2) co_abort.simps(3) co_abort.simps(4) co_state.exhaust split_pairs)
+next
+  case (3 s N s')
+  then show ?case 
+    by (metis (no_types, lifting) co_abort_pa_no_commit co_commit_pa_commit_or_ready co_init_pa_init_or_abort co_state.exhaust co_wait_pa_init_or_abort_or_ready pa_state.distinct(4) pa_state.distinct(8) pa_state.simps(12) pa_state.simps(2) valid_sys.intros(3))
+next
+  case (4 s N s')
+  then show ?case 
+    by (metis co_act_ps_unchanged eq_snd_iff)
+next
+  case (5 s N s')
+  then show ?case 
+    by (metis (no_types, lifting) co_abort_pa_no_commit co_commit_pa_commit_or_ready co_init_pa_init_or_abort co_state.exhaust co_wait_pa_init_or_abort_or_ready pa_state.distinct(1) pa_state.distinct(3) pa_state.distinct(7) pa_state.simps(12) valid_sys.intros(5))
+next
+  case (6 s N x s')
+  then show ?case 
+    by (metis (no_types, lifting) co_abort_pa_init_or_ready_abort co_commit_pa_commit_or_ready co_init_pa_init_or_abort co_state.exhaust co_wait_pa_init_or_abort_or_ready pa_state.distinct(1) pa_state.distinct(3) pa_state.distinct(7) pa_state.simps(12) valid_sys.intros(6))
+qed
 
-fun consistent_pa_states :: "pa_state \<Rightarrow> pa_state \<Rightarrow> bool" where
-  "consistent_pa_states PaCommit PaAbort = False"
-| "consistent_pa_states PaAbort PaCommit = False"
-| "consistent_pa_states _ _ = True"
-
-lemma safety:
+theorem safety:
   assumes "valid_sys s N"
     and "x < N"
     and "y < N"
